Instances/ISAs/DispatchLoopEval.lean
@@ -147,7 +147,7 @@ def exprNodeCount {Reg : Type} : SymExpr Reg → Nat
   | .const _ => 1
   | .reg _ => 1
   | .low32 x | .uext32 x | .sext8to32 x | .sext32to64 x => 1 + exprNodeCount x
-  | .sub32 a b | .shl32 a b | .add64 a b | .sub64 a b
+  | .sub32 a b | .shl32 a b | .and32 a b | .add64 a b | .sub64 a b
   | .xor64 a b | .and64 a b | .or64 a b | .shl64 a b | .shr64 a b =>
     1 + exprNodeCount a + exprNodeCount b
   | .load _ m addr => 1 + memNodeCount m + exprNodeCount addr
@@ -159,7 +159,7 @@ def memNodeCount {Reg : Type} : SymMem Reg → Nat
 def exprUnresolvedLoads {Reg : Type} : SymExpr Reg → Nat
   | .const _ | .reg _ => 0
   | .low32 x | .uext32 x | .sext8to32 x | .sext32to64 x => exprUnresolvedLoads x
-  | .sub32 a b | .shl32 a b | .add64 a b | .sub64 a b
+  | .sub32 a b | .shl32 a b | .and32 a b | .add64 a b | .sub64 a b
   | .xor64 a b | .and64 a b | .or64 a b | .shl64 a b | .shr64 a b =>
     exprUnresolvedLoads a + exprUnresolvedLoads b
   | .load _ m addr => (match m with | .base => 0 | _ => 1) + memUnresolvedLoads m + exprUnresolvedLoads addr
@@ -185,6 +185,7 @@ def exprSummary {Reg : Type} [ToString Reg] : SymExpr Reg → Nat → String
   | .shr64 a b, d => s!"shr({exprSummary a (d-1)},{exprSummary b (d-1)})"
   | .sub32 a b, d => s!"sub32({exprSummary a (d-1)},{exprSummary b (d-1)})"
   | .shl32 a b, d => s!"shl32({exprSummary a (d-1)},{exprSummary b (d-1)})"
+  | .and32 a b, d => s!"and32({exprSummary a (d-1)},{exprSummary b (d-1)})"
   | .load w m addr, d => s!"ld{w.byteCount*8}(mem[{memNodeCount m}],{exprSummary addr (d-1)})"
 end
 
@@ -328,7 +329,7 @@ def simplifyLoadStoreExpr {Reg : Type} [DecidableEq Reg] : SymExpr Reg → SymEx
   | .sext8to32 x => .sext8to32 (simplifyLoadStoreExpr x)
   | .sext32to64 x => .sext32to64 (simplifyLoadStoreExpr x)
   | .sub32 a b => .sub32 (simplifyLoadStoreExpr a) (simplifyLoadStoreExpr b)
-  | .shl32 a b => .shl32 (simplifyLoadStoreExpr a) (simplifyLoadStoreExpr b)
+  | .and32 a b => .and32 (simplifyLoadStoreExpr a) (simplifyLoadStoreExpr b)  | .shl32 a b => .shl32 (simplifyLoadStoreExpr a) (simplifyLoadStoreExpr b)
   | .add64 a b => foldAdd64 (simplifyLoadStoreExpr a) (simplifyLoadStoreExpr b)
   | .sub64 a b => foldSub64 (simplifyLoadStoreExpr a) (simplifyLoadStoreExpr b)
   | .xor64 a b => .xor64 (simplifyLoadStoreExpr a) (simplifyLoadStoreExpr b)
@@ -386,7 +387,7 @@ def simplifyLoadStoreExprR {Reg : Type} [DecidableEq Reg]
   | .sext8to32 x => .sext8to32 (simplifyLoadStoreExprR classify x)
   | .sext32to64 x => .sext32to64 (simplifyLoadStoreExprR classify x)
   | .sub32 a b => .sub32 (simplifyLoadStoreExprR classify a) (simplifyLoadStoreExprR classify b)
-  | .shl32 a b => .shl32 (simplifyLoadStoreExprR classify a) (simplifyLoadStoreExprR classify b)
+  | .and32 a b => .and32 (simplifyLoadStoreExprR classify a) (simplifyLoadStoreExprR classify b)  | .shl32 a b => .shl32 (simplifyLoadStoreExprR classify a) (simplifyLoadStoreExprR classify b)
   | .add64 a b => foldAdd64 (simplifyLoadStoreExprR classify a) (simplifyLoadStoreExprR classify b)
   | .sub64 a b => foldSub64 (simplifyLoadStoreExprR classify a) (simplifyLoadStoreExprR classify b)
   | .xor64 a b => .xor64 (simplifyLoadStoreExprR classify a) (simplifyLoadStoreExprR classify b)
@@ -550,7 +551,7 @@ def canonicalizeExpr {Reg : Type} [Hashable Reg] : SymExpr Reg → SymExpr Reg
     if (hash a') < (hash b') then .or64 a' b' else .or64 b' a'
   | .sub64 a b => .sub64 (canonicalizeExpr a) (canonicalizeExpr b)
   | .sub32 a b => .sub32 (canonicalizeExpr a) (canonicalizeExpr b)
-  | .shl32 a b => .shl32 (canonicalizeExpr a) (canonicalizeExpr b)
+  | .and32 a b => .and32 (canonicalizeExpr a) (canonicalizeExpr b)  | .shl32 a b => .shl32 (canonicalizeExpr a) (canonicalizeExpr b)
   | .shl64 a b => .shl64 (canonicalizeExpr a) (canonicalizeExpr b)
   | .shr64 a b => .shr64 (canonicalizeExpr a) (canonicalizeExpr b)
   | .load w m addr => .load w (canonicalizeMem m) (canonicalizeExpr addr)
@@ -615,6 +616,7 @@ def SymExpr.toSMTLib {Reg : Type} [ToString Reg] : SymExpr Reg → String
   | .sext32to64 e => s!"((_ sign_extend 32) ((_ extract 31 0) {SymExpr.toSMTLib e}))"
   | .sub32 l r => s!"((_ zero_extend 32) (bvsub ((_ extract 31 0) {SymExpr.toSMTLib l}) ((_ extract 31 0) {SymExpr.toSMTLib r})))"
   | .shl32 l r => s!"((_ zero_extend 32) (bvshl ((_ extract 31 0) {SymExpr.toSMTLib l}) ((_ extract 31 0) {SymExpr.toSMTLib r})))"
+  | .and32 l r => s!"((_ zero_extend 32) (bvand ((_ extract 31 0) {SymExpr.toSMTLib l}) ((_ extract 31 0) {SymExpr.toSMTLib r})))"
   | .add64 l r => s!"(bvadd {SymExpr.toSMTLib l} {SymExpr.toSMTLib r})"
   | .sub64 l r => s!"(bvsub {SymExpr.toSMTLib l} {SymExpr.toSMTLib r})"
   | .xor64 l r => s!"(bvxor {SymExpr.toSMTLib l} {SymExpr.toSMTLib r})"
@@ -652,6 +654,7 @@ def SymExpr.collectRegNames {Reg : Type} [ToString Reg] [BEq Reg] [Hashable Reg]
   | .sext32to64 e, s => SymExpr.collectRegNames e s
   | .sub32 l r, s => SymExpr.collectRegNames r (SymExpr.collectRegNames l s)
   | .shl32 l r, s => SymExpr.collectRegNames r (SymExpr.collectRegNames l s)
+  | .and32 l r, s => SymExpr.collectRegNames r (SymExpr.collectRegNames l s)
   | .add64 l r, s => SymExpr.collectRegNames r (SymExpr.collectRegNames l s)
   | .sub64 l r, s => SymExpr.collectRegNames r (SymExpr.collectRegNames l s)
   | .xor64 l r, s => SymExpr.collectRegNames r (SymExpr.collectRegNames l s)
@@ -676,7 +679,7 @@ def SymExpr.hasLoad {Reg : Type} : SymExpr Reg → Bool
   | .load _ _ _ => true
   | .const _ | .reg _ => false
   | .low32 e | .uext32 e | .sext8to32 e | .sext32to64 e => SymExpr.hasLoad e
-  | .sub32 l r | .shl32 l r | .add64 l r | .sub64 l r | .xor64 l r
+  | .sub32 l r | .shl32 l r | .and32 l r | .add64 l r | .sub64 l r | .xor64 l r
   | .and64 l r | .or64 l r | .shl64 l r | .shr64 l r => SymExpr.hasLoad l || SymExpr.hasLoad r
 
 def SymMem.hasLoad {Reg : Type} : SymMem Reg → Bool
@@ -702,6 +705,7 @@ def SymExpr.collectRegsHS {Reg : Type} [BEq Reg] [Hashable Reg]
   | .sext32to64 e, s => SymExpr.collectRegsHS e s
   | .sub32 l r, s => SymExpr.collectRegsHS r (SymExpr.collectRegsHS l s)
   | .shl32 l r, s => SymExpr.collectRegsHS r (SymExpr.collectRegsHS l s)
+  | .and32 l r, s => SymExpr.collectRegsHS r (SymExpr.collectRegsHS l s)
   | .add64 l r, s => SymExpr.collectRegsHS r (SymExpr.collectRegsHS l s)
   | .sub64 l r, s => SymExpr.collectRegsHS r (SymExpr.collectRegsHS l s)
   | .xor64 l r, s => SymExpr.collectRegsHS r (SymExpr.collectRegsHS l s)
@@ -1372,6 +1376,9 @@ def matchTemplateExpr {Reg : Type} [DecidableEq Reg]
     | _ => none
   | .shl32 ta tb => match e with
     | .shl32 ea eb => (matchTemplateExpr bindings ta ea).bind (matchTemplateExpr · tb eb)
+    | _ => none
+  | .and32 ta tb => match e with
+    | .and32 ea eb => (matchTemplateExpr bindings ta ea).bind (matchTemplateExpr · tb eb)
     | _ => none
   | .add64 ta tb => match e with
     | .add64 ea eb => (matchTemplateExpr bindings ta ea).bind (matchTemplateExpr · tb eb)
@@ -3064,7 +3071,7 @@ def exprLoadsViaRegAddr : SymExpr Amd64Reg → Bool
   | .load _ _ addr => addrUsesRegs addr
   | .low32 e | .uext32 e | .sext8to32 e | .sext32to64 e => exprLoadsViaRegAddr e
   | .add64 a b | .sub64 a b | .xor64 a b | .and64 a b | .or64 a b
-  | .sub32 a b | .shl32 a b | .shl64 a b | .shr64 a b => exprLoadsViaRegAddr a || exprLoadsViaRegAddr b
+  | .sub32 a b | .shl32 a b | .and32 a b | .shl64 a b | .shr64 a b => exprLoadsViaRegAddr a || exprLoadsViaRegAddr b
   | _ => false
 where
   /-- Check if an address expression uses registers (for load address chains). -/
@@ -3073,7 +3080,7 @@ where
   | .const _ => false
   | .load _ _ innerAddr => addrUsesRegs innerAddr  -- chained load: check inner address
   | .add64 a b | .sub64 a b | .xor64 a b | .and64 a b | .or64 a b
-  | .sub32 a b | .shl32 a b | .shl64 a b | .shr64 a b => addrUsesRegs a || addrUsesRegs b
+  | .sub32 a b | .shl32 a b | .and32 a b | .shl64 a b | .shr64 a b => addrUsesRegs a || addrUsesRegs b
   | .low32 e | .uext32 e | .sext8to32 e | .sext32to64 e => addrUsesRegs e
 
 /-- Extract a constant (printable char or token code) from a SymExpr. -/
